Changes in the transformation itself and some lemmas proved for the preservation of semantics proof.

Transfromations.v
@@ -9,11 +9,30 @@ Set Implicit Arguments.
 
 Require Export LambdaSemantics.
 
+Definition is_add_zero (t1 t2 : trm) : option trm :=
+  match t1 with
+  | trm_app val_add (val_int 0) => Some t2
+  | _ => None
+  end.
+
+Lemma is_add_zero_some : forall t1 t2 t m1 m2 v,
+  is_add_zero t1 t2 = Some t -> 
+  red m1 (trm_app t1 t2) m2 v -> 
+  red m1 t m2 v.
+Proof. 
+  introv M R. unfolds is_add_zero. 
+  destruct t1; tryfalse. destruct t1_1; tryfalse.
+  destruct v0; tryfalse. destruct p; tryfalse.
+  destruct t1_2; tryfalse. destruct v0; tryfalse.
+  destruct z; tryfalse. inverts M. Search val_add.
+  inverts R. 
+  { inverts H1. inverts H3. }
+  { asserts_rewrite (0 + n2 = n2). math. constructor. }
+Qed.
+
 (* Remove plus zero, i.e. t + 0 = t and 0 + t = t *)
 Fixpoint transf_rm_pz (t:trm) : trm :=
   match t with
-  | trm_app (trm_app val_add (val_int 0)) t1 => transf_rm_pz t1
-  | trm_app (trm_app val_add t1) (val_int 0) => transf_rm_pz t1
   | trm_val v => trm_val v
   | trm_var x => trm_var x
   | trm_fix b1 b2 t1 => trm_fix b1 b2 (transf_rm_pz t1)
@@ -22,11 +41,19 @@ Fixpoint transf_rm_pz (t:trm) : trm :=
   | trm_let b t1 t2 => 
       trm_let b (transf_rm_pz t1) (transf_rm_pz t2)
   | trm_app t1 t2 => 
-      trm_app (transf_rm_pz t1) (transf_rm_pz t2)
+      let t1' := transf_rm_pz t1 in
+      let t2' := transf_rm_pz t2 in
+      match is_add_zero t1' t2' with
+      | Some t => t
+      | None => trm_app t1' t2'
+      end
   | trm_while t1 t2 => trm_while (transf_rm_pz t1) (transf_rm_pz t2)
   | trm_for v t1 t2 t3 => 
       trm_for v t(transf_rm_pz t1) (transf_rm_pz t2) (transf_rm_pz t3)
   end.
+  
+
+Print transf_rm_pz.
 
 Example simple_example_1: 
   transf_rm_pz (val_add (val_int 0) (val_int 5)) = val_int 5.
@@ -34,34 +61,16 @@ Proof.
   simpl. reflexivity.
 Qed.
 
-Example simple_example_2: 
+(*Example simple_example_2: 
   transf_rm_pz (val_add (val_int 5) (val_int 0)) = val_int 5.
 Proof.
   simpl. reflexivity.
-Qed.
+Qed.*)
 
 Lemma simple_examples_generalisation: forall t,
-  transf_rm_pz (val_add t (val_int 0)) = transf_rm_pz t /\
   transf_rm_pz (val_add (val_int 0) t) = transf_rm_pz t.
 Proof.
-  intros t. intuition. destruct t.
-  - destruct v. 
-    + simpl. reflexivity.
-    + simpl. reflexivity.
-    + destruct z.
-       { simpl. reflexivity. }
-       { simpl. reflexivity. }
-       { simpl. reflexivity. }
-    + simpl. reflexivity.
-    + simpl. reflexivity.
-    + simpl. reflexivity.
-  - simpl. reflexivity.
-  - simpl. reflexivity.
-  - simpl. reflexivity.
-  - simpl. reflexivity.
-  - simpl. reflexivity.
-  - simpl. reflexivity.
-  - simpl. reflexivity.
+  intros. simpl. reflexivity.
 Qed.
 
 (* So far we haven't proved anything interesting since the result follows
@@ -69,17 +78,103 @@ Qed.
    computed, their final output and their effect on the state is the same
    as that of the original code transformation. *)
 
-
-
-Theorem transf_preserves_semantics: forall t s1 s2 v,
-  red s1 t s2 v -> red s1 (transf_rm_pz t) s2 v.
-Proof. 
-  intros t s1 s2 v. intros H. 
-  induction t.
-  - simpl. exact H.
-  - simpl. exact H.
-  - admit. (* Fix... *)
-  - admit. (* Ifs. But how do I know t1 is a bool? *)
-  - simpl. applys red_let. apply IHt1. (* Unfinished *) 
+(* I don't think this is right. *)
+Lemma subst_inert_in_red: forall s1 b v t s2 w,
+  red s1 (subst1 b v t) s2 w <-> red s1 t s2 w.
+Proof.
 Admitted.
+
+Definition bind_eq (b1 b2 : bind) : bool :=
+  match b1, b2 with
+  | bind_anon, bind_anon => true
+  | bind_var x1, bind_var x2 => var_eq x1 x2
+  | _, _ => false
+  end.
+
+(*
+Fixpoint subst' (y:var) (w:val) (t:trm) : trm :=
+  let aux := subst' y w in
+  match t with
+  | trm_val v => t
+  | trm_var x => if var_eq x y then w else t
+  | trm_fix f z t1 => t (* TODO *)
+  | trm_if t0 t1 t2 => trm_if (aux t0) (aux t1) (aux t2)
+  | trm_let z t1 t2 => trm_let z (aux t1) (if bind_eq z y then t2 else aux t2)
+  | trm_app t1 t2 => trm_app (aux t1) (aux t2)
+  | trm_while t1 t2 => trm_while (aux t1) (aux t2)
+  | trm_for x t1 t2 t3 => t (* TODO *)
+  end.
+
+Definition subst1' (b:bind) (v:val) (t:trm) : trm :=
+  match b with
+  | bind_anon => t
+  | bind_var x => subst' x v t
+  end.
+*)
+Fixpoint subst1' (b:bind) (w:val) (t:trm) : trm :=
+  let aux := subst1' b w in
+  match t with
+  | trm_val v => t
+  | trm_var x => if bind_eq b x then w else t
+  | trm_fix f z t1 => t (* TODO *)
+  | trm_if t0 t1 t2 => trm_if (aux t0) (aux t1) (aux t2)
+  | trm_let z t1 t2 => trm_let z (aux t1) (if bind_eq z b then t2 else aux t2)
+  | trm_app t1 t2 => trm_app (aux t1) (aux t2)
+  | trm_while t1 t2 => trm_while (aux t1) (aux t2)
+  | trm_for x t1 t2 t3 => t (* TODO *)
+  end.
+
+Axiom subst1_eq_subst1' : subst1 = subst1'.
+
+Lemma transf_subst_commute: forall b v t,
+  subst1 b v (transf_rm_pz t) = transf_rm_pz (subst1 b v t).
+Proof.
+  intros. rewrite subst1_eq_subst1'. 
+  induction t; simpl. (*try solve [fequal; try case_if; auto].*)
+  { auto. }
+  { case_if; simpl; auto. }
+  { admit. }
+  { fequal*. } 
+  { fequal. 
+    { eauto. }
+    { case_if; eauto. }}
+  { rewrite <- IHt1, <- IHt2. admit. }
+  { fequal; eauto. }
+  { admit. }
+Qed.
+
+Lemma red_transf_subst1 : forall m1 m2 b v t w,
+  red m1 (transf_rm_pz (subst1 b v t)) m2 w -> 
+  red m1 (subst1 b v (transf_rm_pz t)) m2 w.
+Proof.
+Admitted.
+
+Theorem red_transf: forall t s1 s2 v,
+  red s1 t s2 v -> red s1 (transf_rm_pz t) s2 v.
+Proof.
+  introv R. induction R; simpl.
+  { constructor. }
+  { admit. }
+  { eapply red_if.
+    { eauto. }
+    { case_if*. } }
+  { applys* red_let. applys* red_transf_subst1.  }
+  { } 
+
+(*
+  intros t s1 s2 v. generalize s1, s2, v.
+  induction t.
+  (* Base cases *)
+  - simpl. trivial.
+  - simpl. trivial.
+  (* Fix *)
+  - admit. 
+  (* If *)
+  - admit.
+  (* Let *) 
+  - simpl. inversion 1. applys red_let. 
+    + apply IHt1 in H6. exact H6.
+    + apply subst_inert_in_red in H7. apply IHt2 in H7. 
+      apply subst_inert_in_red. exact H7.
+Admitted.*)
 
